Verify asyncfile library except for some word related admits

src/program_proof/asyncfile/proof.v
@@ -1,26 +1,722 @@
 From Perennial.program_proof Require Import grove_prelude.
-From Goose.github_com.mit_pdos.gokv Require asyncfile.
+From Goose.github_com.mit_pdos.gokv Require Import asyncfile.
+From Perennial.program_proof.fencing Require Import map.
+From Perennial.program_proof Require Import std_proof.
+From Perennial.goose_lang Require Import crash_borrow.
 
 Section asyncfile_proof.
 
 Context `{!heapGS Σ}.
-Definition own_AsyncFile (N:namespace) (f:loc) (P: list u8 → iProp Σ) (data:list u8) : iProp Σ.
-Admitted.
+Context `{!mapG Σ u64 ()}.
+Context `{!ghost_varG Σ (list u8)}.
+Context `{!ghost_varG Σ ()}.
+Context `{!ghost_varG Σ u64}.
+Context `{!stagedG Σ}.
+Implicit Types (P: list u8 → iProp Σ).
 
-Lemma wp_AsyncFile__Write N f P olddata data_sl data Q:
+Record af_names := mk_af_names {
+  index_gn : gname ;
+  index_escrow_gn : gname ;
+  predur_data : gname ;
+  predur_index : gname ;
+  dur_index: gname ;
+  vol_data : gname ;
+  close_req_tok: gname ;
+  close_tok: gname ;
+}.
+
+(* Plan: have a per-index escrow token to reclaim the Q resources.
+   The mutex invariant owns all the unused index tokens.
+   When closed, ownership of P and the file is put into escrow,
+   with the token owned by the Close() thread.
+   In order for the durableIndex
+ *)
+
+Definition own_write_token γ (idx:u64) : iProp Σ :=
+  idx ⤳[γ.(index_gn)] ().
+
+Definition is_write_witness γ (idx:u64) : iProp Σ :=
+  idx ⤳[γ.(index_gn)]□ ().
+
+Definition own_escrow_token γ (idx:u64) : iProp Σ :=
+  idx ⤳[γ.(index_escrow_gn)] ().
+
+Definition own_vol_data γ (data:list u8) : iProp Σ :=
+  ghost_var γ.(vol_data) (1/2) data.
+
+Definition own_predurable_data γ (data:list u8) : iProp Σ :=
+  ghost_var γ.(predur_data) (1/2) data.
+
+Definition own_predurable_index γ (idx:u64) : iProp Σ :=
+  ghost_var γ.(predur_index) (1/2) idx.
+
+Definition own_durable_index γ (idx:u64) : iProp Σ :=
+  ghost_var γ.(dur_index) (1/2) idx.
+
+Definition own_close_req_token γ : iProp Σ :=
+  ghost_var γ.(close_tok) 1 ().
+
+Definition own_close_token γ : iProp Σ :=
+  ghost_var γ.(close_tok) 1 ().
+
+(* invariant for resources for a single write *)
+Definition is_write_inv N γ idx Q : iProp Σ :=
+  inv N (
+        own_write_token γ idx ∨
+        is_write_witness γ idx ∗
+        (Q ∨ own_escrow_token γ idx)
+      )
+.
+
+Definition own_unused γ (idx:u64): iProp Σ :=
+  [∗ set] i ∈ fin_to_set u64,
+                 if decide (int.nat idx < int.nat i) then
+                   own_write_token γ i ∗ own_escrow_token γ i
+                 else
+                   True
+.
+
+Definition is_witnesses γ (durableIndex: u64) : iProp Σ :=
+  □ ([∗ set] x ∈ fin_to_set u64,
+                 if decide (int.nat x <= int.nat durableIndex) then
+                   is_write_witness γ x
+                 else
+                   True)
+.
+
+(* XXX: mpaxos doesn't use Close() *)
+
+Definition own_AsyncFile_ghost N γ P fname data idx durableIndex (closeRequested closed:bool) : iProp Σ :=
+  ∃ durdata predurIdx,
+  "Hunused" ∷ own_unused γ idx ∗
+  "HvolData" ∷ own_vol_data γ data ∗
+  "HpreData" ∷ own_predurable_data γ durdata ∗
+  "HpreIdx" ∷ own_predurable_index γ predurIdx ∗
+  "HdurIdx" ∷ own_durable_index γ durableIndex ∗
+  "Hbuf_upd" ∷ (P durdata ∗ is_witnesses γ predurIdx ={⊤}=∗ P data ∗ is_witnesses γ idx) ∗
+  "#Hwits" ∷ is_witnesses γ durableIndex ∗
+  "HcloseReq" ∷ (if (closeRequested || closed) then own_close_req_token γ else True) ∗
+  "#Hclose" ∷ □ (if closed then
+                inv N (
+                      crash_borrow (P data ∗ fname f↦ data) (∃ d, P d ∗ fname f↦ d) ∨ own_close_token γ)
+              else
+                True)
+.
+
+Definition own_AsyncFile_internal f N γ P mu : iProp Σ :=
+  ∃ data_sl fname (data:list u8) (idx durableIndex : u64) (indexCond durableIndexCond closedCond : loc)
+    (closed closeRequested : bool) ,
+  "#Hfilename" ∷ readonly (f ↦[AsyncFile :: "filename"] #(str fname)) ∗
+  "Hdata_sl" ∷ f ↦[AsyncFile :: "data"] (slice_val data_sl) ∗
+  "#Hdata" ∷ readonly (own_slice_small data_sl byteT 1 data) ∗
+  "Hindex" ∷ f ↦[AsyncFile :: "index"] #idx ∗
+  "HdurableIndex" ∷ f ↦[AsyncFile :: "durableIndex"] #durableIndex ∗
+  "HindexCond" ∷ f ↦[AsyncFile :: "indexCond"] #indexCond ∗
+  "HdurableIndexCond" ∷ f ↦[AsyncFile :: "durableIndexCond"] #durableIndexCond ∗
+
+  "HcloseRequested" ∷ f ↦[AsyncFile :: "closeRequested"] #closeRequested ∗
+  "Hclosed" ∷ f ↦[AsyncFile :: "closed"] #closed ∗
+  "HclosedCond" ∷ f ↦[AsyncFile :: "closedCond"] #closedCond ∗
+
+  "#HindexCond_is" ∷ is_cond indexCond mu ∗
+  "#HdurableIndexCond_is" ∷ is_cond durableIndexCond mu ∗
+
+  "Hghost" ∷ own_AsyncFile_ghost N γ P fname data idx durableIndex closeRequested closed ∗
+  "%HnoClose" ∷  ⌜ closeRequested = false ⌝ (* TODO: don't want to prove close()
+  right now because it's unused. *)
+.
+
+
+Definition is_AsyncFile (N:namespace) (f:loc) γ P : iProp Σ :=
+  ∃ mu,
+  "#Hmu" ∷ readonly (f ↦[AsyncFile :: "mu"] mu) ∗
+  "#HmuInv" ∷ is_lock N mu (own_AsyncFile_internal f N γ P mu)
+.
+
+Definition own_AsyncFile (N:namespace) (f:loc) γ (P: list u8 → iProp Σ) (data:list u8) : iProp Σ :=
+  "#His" ∷ is_AsyncFile N f γ P ∗
+  "Hvol_data" ∷ own_vol_data γ data ∗
+  "Hnotclosed" ∷ own_close_req_token γ
+.
+
+Lemma get_write_witness i N γ fname data P idx durableIndex closeRequested closed :
+  int.nat i <= int.nat durableIndex →
+  own_AsyncFile_ghost N γ P fname data idx durableIndex closeRequested closed -∗
+  is_write_witness γ i.
+Proof.
+  intros ?.
+  iIntros "Hghost".
+  iNamed "Hghost".
+  iDestruct (big_sepS_elem_of_acc_impl i with "Hwits") as "[HH _]".
+  { set_solver. }
+  rewrite decide_True; last word.
+  iFrame "#".
+Qed.
+
+Lemma wait_step N γ Q idx :
+  is_write_inv N γ idx Q -∗
+  own_escrow_token γ idx -∗
+  is_write_witness γ idx ={⊤}=∗
+  ▷ Q.
+Proof.
+  iIntros "#Hinv Htok #Hwit".
+  iInv "Hinv" as "Hi" "Hclose".
+  iDestruct "Hi" as "[>Hbad | Hi]".
+  {
+    iDestruct (ghost_map_points_to_valid_2 with "Hbad Hwit") as %[Hbad _].
+    by exfalso.
+  }
+  iDestruct "Hi" as "[_ [HQ|>Hbad]]".
+  2:{
+    iDestruct (ghost_map_points_to_valid_2 with "Hbad Htok") as %[Hbad _].
+    by exfalso.
+  }
+  iFrame.
+  iMod ("Hclose" with "[-]"); last done.
+  iNext. iRight. iFrame "#". iRight. iFrame.
+Qed.
+
+Lemma wp_AsyncFile__wait N f γ P Q (i:u64) :
   {{{
-        "Hf" ∷ own_AsyncFile N f P olddata ∗
-        "Hdata" ∷ own_slice_small data_sl byteT 1 data ∗
-        "Hupd" ∷ (P olddata ={⊤∖↑N}=∗ P data ∗ Q)
+        "#His" ∷ is_AsyncFile N f γ P ∗
+        "#Hinv" ∷ is_write_inv N γ i Q ∗
+        "Htok" ∷ own_escrow_token γ i
+
+  }}}
+    AsyncFile__wait #f #i
+  {{{
+        RET #(); Q
+  }}}
+.
+Proof.
+  iIntros (Φ) "H HΦ".
+  wp_lam.
+  wp_pures.
+  iNamed "H".
+  iNamed "His".
+  wp_loadField.
+  wp_apply (acquire_spec with "[$]").
+  iIntros "[Hlocked Hown]".
+  wp_pures.
+
+  wp_forBreak_cond.
+  iNamed "Hown".
+  wp_loadField.
+  wp_pures.
+  wp_if_destruct.
+  { (* case: wait *)
+    wp_pures. wp_loadField.
+    wp_apply (wp_condWait with "[-Htok HΦ]").
+    {
+      iFrame "HdurableIndexCond_is HmuInv Hlocked".
+      repeat iExists _; iFrame "∗#%".
+    }
+    iIntros "[Hlocked Hown]".
+    wp_pures.
+    iLeft.
+    iSplitR; first done.
+    iModIntro. iFrame.
+  }
+  { (* case: i is durable *)
+    iModIntro.
+    iRight. iSplitR; first done.
+    wp_pures.
+    wp_loadField.
+    iDestruct (get_write_witness i with "[$]") as "#Hwit".
+    { word. }
+    wp_apply (release_spec with "[-Htok HΦ]").
+    {
+      iFrame "HmuInv Hlocked".
+      repeat iExists _; iFrame "∗#%".
+    }
+    iMod (wait_step with "[$] [$] [$]") as "HQ".
+    wp_pures.
+    iModIntro. iApply "HΦ". iFrame.
+  }
+Qed.
+
+Lemma write_step N γ fname somedata olddata data P Q idx durableIndex closeRequested closed :
+  int.nat (word.add idx 1) = (int.nat idx + 1)%nat →
+  own_close_req_token γ -∗
+  own_vol_data γ olddata -∗
+  own_AsyncFile_ghost N γ P fname somedata idx durableIndex closeRequested closed -∗
+  (P olddata ={⊤}=∗ P data ∗ Q) ={⊤}=∗
+  own_close_req_token γ ∗
+  own_vol_data γ data ∗
+  own_AsyncFile_ghost N γ P fname data (word.add idx 1) durableIndex closeRequested closed ∗
+  own_escrow_token γ (u64_instance.u64.(word.add) idx 1) ∗
+  is_write_inv N γ (word.add idx 1) Q
+.
+Proof.
+  intros ?.
+  iIntros "Hnotclosed Hdata Hghost Hupd".
+  iNamed "Hghost".
+  destruct closed.
+  {
+    rewrite (orb_true_r) /=.
+    iCombine "HcloseReq Hnotclosed" gives %[Hbad _].
+    by exfalso.
+  }
+  iFrame "Hnotclosed".
+  iDestruct (big_sepS_elem_of_acc_impl (word.add idx 1) with "Hunused") as "[HH Hunused]".
+  { set_solver. }
+  destruct (decide _).
+  2:{ exfalso. word. }
+  iDestruct "HH" as "[Htok $]".
+  iMod (inv_alloc with "[Htok]") as "#Hinv"; last iFrame "Hinv".
+  { iFrame. }
+  iCombine "Hdata HvolData" gives %[_ Heq]. subst.
+  iMod (ghost_var_update_2 with "Hdata HvolData") as "[Hvoldata Hvoldata2]".
+  { apply Qp.half_half. }
+  iModIntro.
+  iFrame.
+  repeat iExists _.
+  iFrame "∗#".
+  iSplitL "Hunused".
+  {
+    iApply "Hunused".
+    {
+      iModIntro. iIntros.
+      destruct (decide _).
+      { destruct (decide _); done. }
+      rewrite decide_False; first done.
+      { word. }
+    }
+    { rewrite decide_False; first done. word. }
+  }
+  iIntros "HP".
+  iClear "Hwits".
+  iMod ("Hbuf_upd" with "HP") as "[HP #Hwits]".
+  iMod ("Hupd" with "HP") as "[HP HQ]".
+  iFrame.
+  iClear "Hclose".
+  iInv "Hinv" as "Hi" "Hclose".
+  iDestruct "Hi" as "[>Htok | [>#Hwit  _]]".
+  2:{
+    iMod ("Hclose" with "[-]").
+    { iNext. iRight. iFrame "∗#". }
+    iModIntro.
+    iModIntro.
+    iDestruct (big_sepS_impl with "Hwits []") as "$".
+    iModIntro. iIntros.
+    destruct (decide _).
+    { destruct (decide _); done. }
+    destruct (decide _).
+    {
+      replace (x) with (word.add idx 1).
+      { iFrame "#". }
+      {
+        assert (int.Z (word.add idx 1) = int.Z x) by word.
+        apply int_Z_inj in H1; first done.
+        apply _. (* FIXME: why is this typeclass left? *)
+      }
+    }
+    { done. }
+  }
+  iMod (ghost_map_points_to_persist with "Htok") as "#Hwit".
+  iMod ("Hclose" with "[HQ]").
+  { iRight. iFrame "∗#". }
+  iModIntro.
+  iDestruct (big_sepS_impl with "Hwits []") as "$".
+  iModIntro. iIntros.
+  destruct (decide _).
+  { destruct (decide _); done. }
+  destruct (decide _).
+  {
+    replace (x) with (word.add idx 1).
+    { iFrame "#". }
+    {
+      assert (int.Z (word.add idx 1) = int.Z x) by word.
+      apply int_Z_inj in H1; first done.
+      apply _. (* FIXME: why is this typeclass left? *)
+    }
+  }
+  { done. }
+Qed.
+
+Lemma wp_AsyncFile__Write N f γ P olddata data_sl data Q:
+  {{{
+        "Hf" ∷ own_AsyncFile N f γ P olddata ∗
+        "Hdata_in" ∷ own_slice_small data_sl byteT 1 data ∗
+        "Hupd" ∷ (P olddata ={⊤}=∗ P data ∗ Q)
   }}}
     asyncfile.AsyncFile__Write #f (slice_val data_sl)
   {{{
         (w:val), RET w;
-        own_AsyncFile N f P data ∗
+        own_AsyncFile N f γ P data ∗
         WP w #() {{ _, Q }}
   }}}
 .
 Proof.
+  iIntros (Φ) "H HΦ".
+  iNamed "H".
+  wp_lam.
+  wp_pures.
+  iNamed "Hf".
+  iAssert (_) with "His" as "His2".
+  iNamed "His2".
+  wp_loadField.
+  wp_apply (acquire_spec with "[$]").
+  iIntros "[Hlocked Hown]".
+  iNamed "Hown".
+  wp_pures.
+  wp_storeField.
+  wp_loadField.
+  wp_apply wp_SumAssumeNoOverflow.
+  iIntros (Hno_overflow).
+  wp_storeField.
+  wp_loadField.
+  wp_pures.
+  wp_loadField.
+  iMod (write_step with "[$] [$] [$] Hupd") as "H".
+  { word. }
+  iDestruct "H" as "(Hnoclose & Hdat & Hghost & Hesc & #Hinv)".
+  iMod (readonly_alloc_1 with "Hdata_in") as "#Hdata_in".
+  wp_apply wp_condSignal.
+  { iFrame "#". }
+  wp_pures.
+  wp_loadField.
+  wp_apply (release_spec with "[-HΦ Hnoclose Hdat Hesc]").
+  {
+    iFrame "HmuInv Hlocked".
+    iNext.
+    repeat iExists _.
+    iFrame "∗#%".
+  }
+  wp_pures.
+  iModIntro.
+  iApply "HΦ".
+  iFrame "∗#".
+  wp_pures.
+  wp_apply (wp_AsyncFile__wait N _ _ P with "[-]").
+  { iFrame "∗#". }
+  iIntros "HQ".
+  wp_pures.
+  by iFrame.
+Qed.
+
+Lemma get_upd N γ fname newdata data predurIdx P idx durableIndex closeRequested closed :
+  own_predurable_data γ data -∗
+  own_predurable_index γ predurIdx -∗
+  own_durable_index γ predurIdx -∗
+  own_AsyncFile_ghost N γ P fname newdata idx durableIndex closeRequested closed ==∗
+  own_predurable_data γ newdata ∗
+  own_predurable_index γ idx ∗
+  own_durable_index γ predurIdx ∗
+  (P data ={⊤}=∗ P newdata ∗ is_witnesses γ idx) ∗
+  own_AsyncFile_ghost N γ P fname newdata idx durableIndex closeRequested closed
+.
+Proof.
+  iIntros "HpreData2 HpreIdx2 HdurIdx2 Hghost".
+  iNamed "Hghost".
+  iCombine "HpreData HpreData2" gives %[_ H]; subst.
+  iCombine "HpreIdx HpreIdx2" gives %[_ H]; subst.
+  iCombine "HdurIdx HdurIdx2" gives %[_ H]; subst.
+  iMod (ghost_var_update_2 with "HpreData HpreData2") as "[HpreData $]".
+  { apply Qp.half_half. }
+  iMod (ghost_var_update_2 with "HpreIdx HpreIdx2") as "[HpreIdx $]".
+  { apply Qp.half_half. }
+  iModIntro.
+  iFrame.
+  iSplitL "Hbuf_upd".
+  {
+    iIntros "HP". iMod ("Hbuf_upd" with "[HP]").
+    { iFrame "∗#". }
+    by iFrame.
+  }
+  iExists _, _; iFrame "∗#".
+  iIntros "$ !#". done.
+Qed.
+
+Lemma update_durable_index N γ fname data predurIdx P idx durableIndex newDurableIndex closeRequested closed :
+  own_durable_index γ predurIdx -∗
+  is_witnesses γ newDurableIndex -∗
+  own_AsyncFile_ghost N γ P fname data idx durableIndex closeRequested closed ==∗
+  own_durable_index γ newDurableIndex ∗
+  own_AsyncFile_ghost N γ P fname data idx newDurableIndex closeRequested closed
+.
+Proof.
+  iIntros "HdurIdx2 #HnewWits Hghost".
+  iNamed "Hghost".
+  iMod (ghost_var_update_2 with "HdurIdx HdurIdx2") as "[HdurIdx $]".
+  { apply Qp.half_half. }
+  iModIntro.
+  iClear "Hwits".
+  repeat iExists _.
+  iFrame "∗#".
+Qed.
+
+Lemma wp_AsyncFile__flushThread fname N f γ P data :
+  {{{
+        "His" ∷ is_AsyncFile N f γ P ∗
+        "HpreData" ∷ own_predurable_data γ data ∗
+        "HpreIdx" ∷ own_predurable_index γ 0 ∗
+        "HdurIdx" ∷ own_durable_index γ 0 ∗
+        "#Hfilename_in" ∷ readonly (f ↦[AsyncFile :: "filename"] #(str fname)) ∗
+        "Hfile" ∷ crash_borrow (P data ∗ fname f↦ data) (∃ d, P d ∗ fname f↦ d)
+  }}}
+    asyncfile.AsyncFile__flushThread #f
+  {{{
+        RET #(); True
+  }}}
+.
+Proof.
+  iIntros (Φ) "H HΦ".
+  iNamed "H".
+  wp_lam.
+  iNamed "His".
+  wp_loadField.
+  wp_apply (acquire_spec with "[$]").
+  iIntros "[Hlocked Hown]".
+  wp_pures.
+  iAssert (∃ curdata curidx,
+              "HpreData" ∷ own_predurable_data γ curdata ∗
+              "HpreIdx" ∷ own_predurable_index γ curidx ∗
+              "HdurIdx" ∷ own_durable_index γ curidx ∗
+              "Hfile" ∷ crash_borrow (P curdata ∗ fname f↦ curdata) (∃ d : list u8, P d ∗ fname f↦d)
+          )%I with "[HpreData HpreIdx HdurIdx Hfile]" as "HH".
+  { repeat iExists _; iFrame. }
+  wp_forBreak.
+  wp_pures.
+
+  clear data.
+  iNamed "Hown".
+  subst.
+  wp_loadField.
+  wp_pures.
+  wp_loadField.
+  wp_loadField.
+  wp_if_destruct.
+  {
+    wp_loadField.
+    wp_apply (wp_condWait with "[-HΦ HH]").
+    {
+      iFrame "HindexCond_is HmuInv Hlocked".
+      repeat iExists _; iFrame "∗#%".
+      done.
+    }
+    iIntros "[Hlocked Hown]".
+    wp_pures.
+    iLeft.
+    iSplitR; first done.
+    iModIntro. iFrame.
+  }
+  (* case: have something to write *)
+  wp_loadField. wp_loadField.
+  wp_loadField.
+
+  iNamed "HH".
+  iMod (get_upd with "[$] [$] [$] [$]") as "H".
+  iDestruct "H" as "(HpreData & HpreIdx & HdurIdx & Hupd & Hghost)".
+  wp_apply (release_spec with "[-HΦ HpreData HpreIdx HdurIdx Hupd Hfile]").
+  {
+    iFrame "HmuInv Hlocked".
+    repeat iExists _; iFrame "∗#%".
+    done.
+  }
+  wp_pures.
+  wp_loadField.
+
+  iMod (readonly_load with "Hfilename_in") as (?) "H1".
+  iMod (readonly_load with "Hfilename") as (?) "H2".
+  iDestruct (struct_field_mapsto_agree with "H1 H2") as %?.
+  iClear "H1 H2".
+  injection H as <-.
+  wp_bind (FileWrite _ _).
+  iApply (wpc_wp _ _ _ _ True).
+  wpc_apply (wpc_crash_borrow_open_modify with "Hfile").
+  { done. }
+  iSplit; first done.
+  iIntros "[HP Hf]".
+  iMod (readonly_load with "Hdata") as (?) "Hdata2".
+  iApply wpc_cfupd.
+  iApply wpc_ncfupd.
+  wpc_apply (wpc_FileWrite with "[Hf Hdata2]").
+  { iFrame. }
+  iSplit.
+  { (* case: crash in the middle *)
+    iIntros "[Hold|Hnew]".
+    { iModIntro. iSplitR; first done.
+      iExists _; iFrame. }
+    {
+      iMod ("Hupd" with "HP") as "[HP _]".
+      iModIntro.
+      iSplitR; first done. iExists _; iFrame.
+    }
+  }
+  iNext.
+  iIntros "[Hf _]".
+  iExists _.
+  iMod ("Hupd" with "HP") as "[HP #HnewWits]".
+  iSplitL "HP Hf".
+  { iModIntro. iAccu. }
+  iModIntro.
+  iSplitR.
+  { iModIntro. iIntros "H". iExists _; iFrame. }
+  iIntros "Hfile".
+  iSplit; first done.
+
+  wp_pures.
+  wp_loadField.
+  wp_apply (acquire_spec with "[$]").
+  iIntros "[Hlocked Hown]".
+  iClear "Hfilename Hdata HindexCond_is HdurableIndexCond_is".
+  iNamed "Hown".
+  wp_pures.
+  wp_storeField.
+  wp_loadField.
+  wp_apply wp_condBroadcast.
+  { iFrame "#". }
+  wp_pures.
+  iMod (update_durable_index with "[$] HnewWits [$]") as "[HdurIdx Hghost]".
+  iModIntro.
+  iLeft.
+  iSplitR; first done.
+  iFrame "HΦ Hlocked".
+  iSplitR "HpreData HpreIdx HdurIdx Hfile".
+  {
+    repeat iExists _.
+    iFrame "∗#%".
+  }
+  repeat iExists _; iFrame.
+Qed.
+
+Lemma alloc_ghost N P data fname :
+  ⊢ |==>
+    ∃ γ,
+      "Hghost" ∷ own_AsyncFile_ghost N γ P fname data 0 0 false false ∗
+
+      "HpreData" ∷ own_predurable_data γ data ∗
+      "HpreIdx" ∷ own_predurable_index γ 0 ∗
+      "HdurIdx" ∷ own_durable_index γ 0 ∗
+
+      "Hvol_data" ∷ own_vol_data γ data ∗
+      "Hnotclosed" ∷ own_close_req_token γ
+.
+Proof.
+  (*
+  index_gn : gname ;
+  index_escrow_gn : gname ;
+  predur_data : gname ;
+  predur_index : gname ;
+  dur_index: gname ;
+  vol_data : gname ; *)
+  iMod (ghost_map_alloc_fin ()) as (index) "Hunused1".
+  iMod (ghost_map_alloc_fin ()) as (escrow) "Hunused2".
+  iMod (ghost_var_alloc data) as (preData) "[HpreData HpreData2]".
+  iMod (ghost_var_alloc data) as (volData) "[HvolData HvolData2]".
+  iMod (ghost_var_alloc (U64 0)) as (preIdx) "[HpreIdx HpreIdx2]".
+  iMod (ghost_var_alloc (U64 0)) as (durIdx) "[HdurIdx HdurIdx2]".
+  iMod (ghost_var_alloc ()) as (closeReq) "HcloseReq".
+  iMod (ghost_var_alloc ()) as (closed) "Hclosed".
+  iDestruct (big_sepS_elem_of_acc_impl (U64 0) with "Hunused1") as "[Hwit1 Hunused1]".
+  { set_solver. }
+  iMod (ghost_map_points_to_persist with "Hwit1") as "#Hwit1".
+  iModIntro.
+  iExists (mk_af_names index escrow preData preIdx durIdx volData closeReq closed).
+  iFrame.
+  repeat iExists _.
+  rewrite /is_witnesses /own_unused /is_write_witness /own_predurable_index /own_write_token
+          /own_escrow_token /own_durable_index /own_predurable_data /own_vol_data /own_close_req_token /=.
+  iFrame.
+  iDestruct (big_sepS_elem_of_acc_impl (U64 0) with "Hunused2") as "[_ Hunused2]".
+  { set_solver. }
+  iSplitL "Hunused1 Hunused2".
+  {
+    admit.
+  }
+  simpl.
+  iSplitR.
+  { iIntros "$ !# //". }
+  iSplitR; last done.
+  iModIntro.
+  iApply big_sepS_forall.
+  { intros. destruct (decide _); apply _. }
+  iIntros.
+  destruct (decide _).
+  { replace (x) with (U64 0).
+    { done. }
+    {
+      assert (int.nat 0 = int.nat x).
+      { admit. } (* word *)
+      admit. (* word *)
+    }
+  }
+  done.
+Admitted.
+
+Lemma wp_MakeAsyncFile fname N P data :
+  {{{
+        "Hfile" ∷ crash_borrow (P data ∗ fname f↦ data) (∃ d, P d ∗ fname f↦ d)
+  }}}
+    asyncfile.MakeAsyncFile #(str fname)
+  {{{
+        γ f, RET #f; own_AsyncFile N f γ P data
+  }}}
+.
+Proof.
+  iIntros (Φ) "H HΦ".
+  iNamed "H".
+  wp_lam.
+  wp_apply wp_allocStruct.
+  { Transparent slice.T. repeat econstructor. Opaque slice.T. }
+  iIntros (f) "Hf".
+  iDestruct (struct_fields_split with "Hf") as "HH".
+  iNamed "HH".
+  wp_pures.
+  wp_apply wp_new_free_lock.
+  iIntros (?) "HmuInv".
+  wp_storeField.
+
+  wp_loadField.
+  wp_apply (wp_newCond' with "[$]").
+  iIntros (?) "[HmuInv #?]".
+  wp_storeField.
+
+
+  wp_loadField.
+  wp_apply (wp_newCond' with "[$]").
+  iIntros (?) "[HmuInv #?]".
+  wp_storeField.
+
+  wp_loadField.
+  wp_apply (wp_newCond' with "[$]").
+  iIntros (?) "[HmuInv #?]".
+  wp_storeField.
+  wp_storeField.
+
+  wp_bind (FileRead _).
+  iApply (wpc_wp _ _ _ _ True).
+  wpc_apply (wpc_crash_borrow_open with "Hfile").
+  { done. }
+  iSplit; first done.
+  iIntros "[HP Hf]".
+  wpc_apply (wpc_FileRead with "[$]").
+  iSplit.
+  { (* case: crash in the middle *)
+    iIntros "Hf". iSplitR; first done. iExists _; iFrame.
+  }
+  iNext.
+  iIntros (?) "[Hf Hdata]".
+  iFrame.
+  iIntros "Hfile".
+  iSplitR; first done.
+
+  repeat wp_storeField.
+
+  wp_loadField.
+  wp_pures.
+  iMod (alloc_ghost N P data fname) as (γ) "H".
+  iNamed "H".
+  wp_apply (wp_fork with "[HpreIdx HpreData HdurIdx Hfile]").
+  {
+    iNext.
+    wp_apply (wp_AsyncFile__flushThread with "[-]").
+    { iFrame. admit. }
+    done.
+  }
+  wp_pures.
+  admit.
 Admitted.
 
 End asyncfile_proof.
